<?xml version="1.0"?>
<rdf:RDF xmlns="https://w3id.org/ontoim/"
     xml:base="https://w3id.org/ontoim/"
     xmlns:cc="http://creativecommons.org/licenses/by/"
     xmlns:dc="http://purl.org/dc/elements/1.1/"
     xmlns:l0="https://w3id.org/italia/onto/l0/"
     xmlns:ns="http://www.w3.org/2006/vcard/ns#"
     xmlns:cis="http://dati.beniculturali.it/cis/"
     xmlns:dct="http://purl.org/dc/terms/"
     xmlns:owl="http://www.w3.org/2002/07/owl#"
     xmlns:rdf="http://www.w3.org/1999/02/22-rdf-syntax-ns#"
     xmlns:sdo="https://schema.org/"
     xmlns:xml="http://www.w3.org/XML/1998/namespace"
     xmlns:xsd="http://www.w3.org/2001/XMLSchema#"
     xmlns:dcat="http://www.w3.org/ns/dcat#"
     xmlns:foaf="http://xmlns.com/foaf/0.1/"
     xmlns:prov="http://www.w3.org/ns/prov#"
     xmlns:rdfs="http://www.w3.org/2000/01/rdf-schema#"
     xmlns:w3id="https://w3id.org/"
     xmlns:acapit="https://w3id.org/italia/onto/AccessCondition/"
     xmlns:chapit="https://w3id.org/italia/onto/CulturalHeritage/"
     xmlns:muapit="https://w3id.org/italia/onto/MU/"
     xmlns:pcapit="https://w3id.org/italia/onto/PublicContract/"
     xmlns:roapit="https://w3id.org/italia/onto/RO/"
     xmlns:rtapit="https://w3id.org/italia/onto/Route/"
     xmlns:smapit="https://w3id.org/italia/onto/SM/"
     xmlns:tiapit="https://w3id.org/italia/onto/TI/"
     xmlns:trapit="https://w3id.org/italia/onto/Transparency/"
     xmlns:aopapit="https://w3id.org/italia/onto/AtlasOfPaths/"
     xmlns:clvapit="https://w3id.org/italia/onto/CLV/"
     xmlns:covapit="https://w3id.org/italia/onto/COV/"
     xmlns:cpvapit="https://w3id.org/italia/onto/CPV/"
     xmlns:herapit="https://w3id.org/italia/onto/HER/"
     xmlns:iotapit="https://w3id.org/italia/onto/IoT/"
     xmlns:poiapit="https://w3id.org/italia/onto/POI/"
     xmlns:potapit="https://w3id.org/italia/onto/POT/"
     xmlns:prjapit="https://w3id.org/italia/onto/Project/"
     xmlns:accoapit="https://w3id.org/italia/onto/ACCO/"
     xmlns:admsapit="https://w3id.org/italia/onto/ADMS/"
     xmlns:cpevapit="https://w3id.org/italia/onto/CPEV/"
     xmlns:cpsvapit="https://w3id.org/italia/onto/CPSV/"
     xmlns:langapit="https://w3id.org/italia/onto/Language/"
     xmlns:parkapit="https://w3id.org/italia/onto/PARK/"
     xmlns:indicator="https://w3id.org/italia/onto/Indicator/">
    <owl:Ontology rdf:about="https://w3id.org/ontoim">
        <owl:imports rdf:resource="https://w3id.org/italia/onto/ACCO"/>
        <owl:imports rdf:resource="https://w3id.org/italia/onto/ADMS"/>
        <owl:imports rdf:resource="https://w3id.org/italia/onto/AccessCondition"/>
        <owl:imports rdf:resource="https://w3id.org/italia/onto/CLV"/>
        <owl:imports rdf:resource="https://w3id.org/italia/onto/COV"/>
        <owl:imports rdf:resource="https://w3id.org/italia/onto/CPEV"/>
        <owl:imports rdf:resource="https://w3id.org/italia/onto/CPSV"/>
        <owl:imports rdf:resource="https://w3id.org/italia/onto/CPV"/>
        <owl:imports rdf:resource="https://w3id.org/italia/onto/IoT"/>
        <owl:imports rdf:resource="https://w3id.org/italia/onto/MU"/>
        <owl:imports rdf:resource="https://w3id.org/italia/onto/POI"/>
        <owl:imports rdf:resource="https://w3id.org/italia/onto/POT"/>
        <owl:imports rdf:resource="https://w3id.org/italia/onto/PublicContract"/>
        <owl:imports rdf:resource="https://w3id.org/italia/onto/SM"/>
        <owl:imports rdf:resource="https://w3id.org/italia/onto/TI"/>
        <owl:imports rdf:resource="https://w3id.org/italia/onto/l0"/>
        <dct:accrualPeriodicity rdf:resource="http://publications.europa.eu/resource/authority/frequency/IRREG"/>
        <dct:created rdf:datatype="http://www.w3.org/2001/XMLSchema#date">2022-09-24</dct:created>
        <dct:creator rdf:resource="https://orcid.org/0000-0002-6249-0899"/>
        <dct:description xml:lang="it">Questa ontologia, unita alle ontologie della rete italiana OntoPiA, permette di modellare la realtà di un Comune. Include eventi, associazioni, imprese, scuole, ospedali, aree verdi, piante, segnaletica stradale, osservazioni sul traffico, incidenti stradali e statistiche demografiche.</dct:description>
        <dct:description xml:lang="en">This ontology, combined with ontologies from the Italian OntoPiA network, makes it possible to model the reality of a municipality. It includes events, associations, businesses, schools, hospitals, green areas, plants, street signs, traffic observations, traffic accidents and demographic statistics.</dct:description>
        <dct:issued rdf:datatype="http://www.w3.org/2001/XMLSchema#date">2022-09-24</dct:issued>
        <dct:language rdf:resource="http://publications.europa.eu/resource/authority/language/ENG"/>
        <dct:language rdf:resource="http://publications.europa.eu/resource/authority/language/ITA"/>
        <dct:license rdf:resource="http://creativecommons.org/licenses/by/4.0"/>
        <dct:rightsHolder rdf:resource="https://orcid.org/0000-0002-6249-0899"/>
        <dct:title xml:lang="en">Ontology for Italian Municipalities</dct:title>
        <owl:versionInfo rdf:datatype="http://www.w3.org/2000/01/rdf-schema#Literal">0.1</owl:versionInfo>
        <dcat:accessURL rdf:resource="https://github.com/luca-martinelli-09/ontoim/"/>
        <dcat:contactPoint rdf:resource="https://orcid.org/0000-0002-6249-0899"/>
        <dcat:downloadURL rdf:resource="https://raw.githubusercontent.com/luca-martinelli-09/ontoim/master/ontology/latest/OntoIM.rdf"/>
        <dcat:theme rdf:resource="http://publications.europa.eu/resource/authority/data-theme/TECH"/>
        <sdo:image rdf:resource="https://raw.githubusercontent.com/luca-martinelli-09/ontoim/master/ontology/latest/OntoMunicipality.svg"/>
        <admsapit:acronym>OntoIM</admsapit:acronym>
        <admsapit:prefix>ontoim</admsapit:prefix>
        <admsapit:target xml:lang="en">Citizens</admsapit:target>
        <admsapit:target xml:lang="it">Cittadini</admsapit:target>
        <admsapit:target xml:lang="en">Companies</admsapit:target>
        <admsapit:target xml:lang="it">Imprese</admsapit:target>
        <admsapit:target xml:lang="it">Pubbliche Amministrazioni</admsapit:target>
        <admsapit:target xml:lang="en">Public Organizations</admsapit:target>
    </owl:Ontology>
    


    <!-- 
    ///////////////////////////////////////////////////////////////////////////////////////
    //
    // Annotation properties
    //
    ///////////////////////////////////////////////////////////////////////////////////////
     -->

    


    <!-- http://purl.org/dc/terms/created -->

    <owl:AnnotationProperty rdf:about="http://purl.org/dc/terms/created"/>
    


    <!-- https://schema.org/affiliation -->

    <owl:AnnotationProperty rdf:about="https://schema.org/affiliation"/>
    


    <!-- https://schema.org/email -->

    <owl:AnnotationProperty rdf:about="https://schema.org/email"/>
    


    <!-- https://schema.org/identifier -->

    <owl:AnnotationProperty rdf:about="https://schema.org/identifier"/>
    


    <!-- https://schema.org/image -->

    <owl:AnnotationProperty rdf:about="https://schema.org/image"/>
    


    <!-- https://schema.org/name -->

    <owl:AnnotationProperty rdf:about="https://schema.org/name"/>
    


    <!-- https://schema.org/url -->

    <owl:AnnotationProperty rdf:about="https://schema.org/url"/>
    


    <!-- 
    ///////////////////////////////////////////////////////////////////////////////////////
    //
    // Object Properties
    //
    ///////////////////////////////////////////////////////////////////////////////////////
     -->

    


    <!-- https://w3id.org/ontoim/hasCivilStatusCategory -->

    <owl:ObjectProperty rdf:about="https://w3id.org/ontoim/hasCivilStatusCategory">
        <rdfs:domain>
            <owl:Class>
                <owl:unionOf rdf:parseType="Collection">
                    <rdf:Description rdf:about="https://w3id.org/ontoim/CivilStatus"/>
                    <rdf:Description rdf:about="https://w3id.org/ontoim/CivilStatusEvent"/>
                </owl:unionOf>
            </owl:Class>
        </rdfs:domain>
        <rdfs:range rdf:resource="https://w3id.org/ontoim/CivilStatusCategory"/>
        <rdfs:label xml:lang="it">ha categoria di stato civile</rdfs:label>
        <rdfs:label xml:lang="en">has civil status category</rdfs:label>
    </owl:ObjectProperty>
    


    <!-- https://w3id.org/ontoim/hasDemographicEvent -->

    <owl:ObjectProperty rdf:about="https://w3id.org/ontoim/hasDemographicEvent">
        <owl:inverseOf rdf:resource="https://w3id.org/ontoim/isDemographicEventFor"/>
        <rdfs:domain rdf:resource="http://www.w3.org/2002/07/owl#Thing"/>
        <rdfs:range rdf:resource="https://w3id.org/ontoim/DemographicEvent"/>
        <rdfs:label xml:lang="it">ha evento demografico</rdfs:label>
        <rdfs:label xml:lang="en">has demographic event</rdfs:label>
    </owl:ObjectProperty>
    


    <!-- https://w3id.org/ontoim/hasDemographicObservation -->

    <owl:ObjectProperty rdf:about="https://w3id.org/ontoim/hasDemographicObservation">
        <owl:inverseOf rdf:resource="https://w3id.org/ontoim/isDemographicObservationFor"/>
        <rdfs:domain rdf:resource="http://www.w3.org/2002/07/owl#Thing"/>
        <rdfs:range rdf:resource="https://w3id.org/ontoim/DemographicObservation"/>
        <rdfs:label xml:lang="it">ha osservazione demografica</rdfs:label>
        <rdfs:label xml:lang="en">has demographic observation</rdfs:label>
    </owl:ObjectProperty>
    


    <!-- https://w3id.org/ontoim/hasDemographicReference -->

    <owl:ObjectProperty rdf:about="https://w3id.org/ontoim/hasDemographicReference">
        <rdfs:domain>
            <owl:Class>
                <owl:unionOf rdf:parseType="Collection">
                    <rdf:Description rdf:about="https://w3id.org/ontoim/DemographicEvent"/>
                    <rdf:Description rdf:about="https://w3id.org/ontoim/DemographicObservation"/>
                </owl:unionOf>
            </owl:Class>
        </rdfs:domain>
        <rdfs:range>
            <owl:Class>
                <owl:unionOf rdf:parseType="Collection">
                    <rdf:Description rdf:about="https://w3id.org/italia/onto/CPV/Family"/>
                    <rdf:Description rdf:about="https://w3id.org/italia/onto/CPV/Person"/>
                </owl:unionOf>
            </owl:Class>
        </rdfs:range>
        <rdfs:label xml:lang="it">ha riferimento demografico</rdfs:label>
        <rdfs:label xml:lang="en">has demographic reference</rdfs:label>
    </owl:ObjectProperty>
    


    <!-- https://w3id.org/ontoim/hasEmployees -->

    <owl:ObjectProperty rdf:about="https://w3id.org/ontoim/hasEmployees">
        <rdfs:subPropertyOf rdf:resource="https://w3id.org/ontoim/hasDemographicObservation"/>
        <rdfs:domain rdf:resource="https://w3id.org/italia/onto/COV/Organization"/>
        <rdfs:range rdf:resource="https://w3id.org/ontoim/Employees"/>
        <rdfs:label xml:lang="it">ha dipendenti</rdfs:label>
        <rdfs:label xml:lang="en">has employees</rdfs:label>
    </owl:ObjectProperty>
    


    <!-- https://w3id.org/ontoim/hasLocalUnitAddress -->

    <owl:ObjectProperty rdf:about="https://w3id.org/ontoim/hasLocalUnitAddress">
        <rdfs:subPropertyOf rdf:resource="https://w3id.org/italia/onto/CLV/hasAddress"/>
        <rdfs:domain rdf:resource="https://w3id.org/italia/onto/COV/Organization"/>
        <rdfs:range rdf:resource="https://w3id.org/italia/onto/CLV/Address"/>
        <rdfs:comment xml:lang="it">Questa proprietà rappresenta l&apos;indirizzo di un&apos;unità locale o sede staccata di un&apos;organizzazione.</rdfs:comment>
        <rdfs:comment xml:lang="en">This property represents the address of a local unit or branch office of an organization.</rdfs:comment>
        <rdfs:label xml:lang="it">ha indirizzo dell&apos;unità locale</rdfs:label>
        <rdfs:label xml:lang="en">has local unit address</rdfs:label>
    </owl:ObjectProperty>
    


    <!-- https://w3id.org/ontoim/hasSpatialDelimitation -->

    <owl:ObjectProperty rdf:about="https://w3id.org/ontoim/hasSpatialDelimitation">
        <rdfs:domain rdf:resource="http://www.w3.org/2002/07/owl#Thing"/>
        <rdfs:range rdf:resource="https://w3id.org/italia/onto/CLV/SpatialObject"/>
        <rdfs:label xml:lang="it">ha delimitazione spaziale</rdfs:label>
        <rdfs:label xml:lang="en">has spatial delimitation</rdfs:label>
    </owl:ObjectProperty>
    


    <!-- https://w3id.org/ontoim/hasTouristType -->

    <owl:ObjectProperty rdf:about="https://w3id.org/ontoim/hasTouristType">
        <rdfs:domain rdf:resource="https://w3id.org/ontoim/Tourists"/>
        <rdfs:range rdf:resource="https://w3id.org/ontoim/TouristType"/>
        <rdfs:label xml:lang="it">ha tipo di turista</rdfs:label>
        <rdfs:label xml:lang="en">has tourist type</rdfs:label>
    </owl:ObjectProperty>
    


    <!-- https://w3id.org/ontoim/isDemographicEventFor -->

    <owl:ObjectProperty rdf:about="https://w3id.org/ontoim/isDemographicEventFor">
        <rdfs:domain rdf:resource="https://w3id.org/ontoim/DemographicEvent"/>
        <rdfs:range rdf:resource="http://www.w3.org/2002/07/owl#Thing"/>
        <rdfs:label xml:lang="en">is demographic event for</rdfs:label>
        <rdfs:label xml:lang="it">è evento demografico per</rdfs:label>
    </owl:ObjectProperty>
    


    <!-- https://w3id.org/ontoim/isDemographicObservationFor -->

    <owl:ObjectProperty rdf:about="https://w3id.org/ontoim/isDemographicObservationFor">
        <rdfs:domain rdf:resource="https://w3id.org/ontoim/DemographicObservation"/>
        <rdfs:range rdf:resource="http://www.w3.org/2002/07/owl#Thing"/>
        <rdfs:label xml:lang="en">is demographic observation for</rdfs:label>
        <rdfs:label xml:lang="it">è osservazione demografica per</rdfs:label>
    </owl:ObjectProperty>
    


    <!-- https://w3id.org/ontoim/ownedBy -->

    <owl:ObjectProperty rdf:about="https://w3id.org/ontoim/ownedBy">
        <owl:inverseOf rdf:resource="https://w3id.org/ontoim/ownsAccessiblePoI"/>
        <rdfs:domain rdf:resource="https://w3id.org/ontoim/AccessiblePointOfInterest"/>
        <rdfs:range rdf:resource="https://w3id.org/italia/onto/COV/Organization"/>
        <rdfs:label xml:lang="en">owned by</rdfs:label>
        <rdfs:label xml:lang="it">posseduto da</rdfs:label>
    </owl:ObjectProperty>
    


    <!-- https://w3id.org/ontoim/ownsAccessiblePoI -->

    <owl:ObjectProperty rdf:about="https://w3id.org/ontoim/ownsAccessiblePoI">
        <rdfs:domain rdf:resource="https://w3id.org/italia/onto/COV/Organization"/>
        <rdfs:range rdf:resource="https://w3id.org/ontoim/AccessiblePointOfInterest"/>
        <rdfs:label xml:lang="en">owns accessible point of interest</rdfs:label>
        <rdfs:label xml:lang="it">possiede un punto di interesse accessibile</rdfs:label>
    </owl:ObjectProperty>
    


    <!-- https://w3id.org/ontoim/providesService -->

    <owl:ObjectProperty rdf:about="https://w3id.org/ontoim/providesService">
        <rdfs:domain rdf:resource="https://w3id.org/italia/onto/COV/Organization"/>
        <rdfs:range rdf:resource="https://w3id.org/italia/onto/CPSV/Service"/>
        <rdfs:label xml:lang="it">offre un servizio</rdfs:label>
        <rdfs:label xml:lang="en">provides service</rdfs:label>
    </owl:ObjectProperty>
    


    <!-- 
    ///////////////////////////////////////////////////////////////////////////////////////
    //
    // Data properties
    //
    ///////////////////////////////////////////////////////////////////////////////////////
     -->

    


    <!-- https://w3id.org/ontoim/bankruptcyDate -->

    <owl:DatatypeProperty rdf:about="https://w3id.org/ontoim/bankruptcyDate">
        <rdfs:subPropertyOf rdf:resource="https://w3id.org/italia/onto/TI/date"/>
        <rdfs:domain rdf:resource="https://w3id.org/italia/onto/COV/Organization"/>
        <rdfs:range rdf:resource="http://www.w3.org/2001/XMLSchema#date"/>
        <rdfs:comment xml:lang="it">Questa proprietà rappresenta la data in cui un&apos;organizzazione va in bancarotta.</rdfs:comment>
        <rdfs:comment xml:lang="en">This property represents the date on which an organization goes bankrupt.</rdfs:comment>
        <rdfs:label xml:lang="en">bankruptcy date</rdfs:label>
        <rdfs:label xml:lang="it">data di bancarotta</rdfs:label>
    </owl:DatatypeProperty>
    


    <!-- https://w3id.org/ontoim/endActivityDate -->

    <owl:DatatypeProperty rdf:about="https://w3id.org/ontoim/endActivityDate">
        <rdfs:subPropertyOf rdf:resource="https://w3id.org/italia/onto/TI/date"/>
        <rdfs:domain rdf:resource="https://w3id.org/italia/onto/COV/Organization"/>
        <rdfs:range rdf:resource="http://www.w3.org/2001/XMLSchema#date"/>
        <rdfs:comment xml:lang="it">Questa proprietà rappresenta la data in cui un&apos;organizzazione chiude.</rdfs:comment>
        <rdfs:comment xml:lang="en">This property represents the date on which an organization closes.</rdfs:comment>
        <rdfs:label xml:lang="it">data di fine attività</rdfs:label>
        <rdfs:label xml:lang="en">end activity date</rdfs:label>
    </owl:DatatypeProperty>
    


    <!-- https://w3id.org/ontoim/liquidationDate -->

    <owl:DatatypeProperty rdf:about="https://w3id.org/ontoim/liquidationDate">
        <rdfs:subPropertyOf rdf:resource="https://w3id.org/italia/onto/TI/date"/>
        <rdfs:domain rdf:resource="https://w3id.org/italia/onto/COV/Organization"/>
        <rdfs:range rdf:resource="http://www.w3.org/2001/XMLSchema#date"/>
        <rdfs:comment xml:lang="it">Questa proprietà rappresenta la data in cui un&apos;organizzazione viene liquidata.</rdfs:comment>
        <rdfs:comment xml:lang="en">This property represents the date on which an organization is liquidated.</rdfs:comment>
        <rdfs:label xml:lang="it">data di liquidazione</rdfs:label>
        <rdfs:label xml:lang="en">liquidation date</rdfs:label>
    </owl:DatatypeProperty>
    


    <!-- https://w3id.org/ontoim/value -->

    <owl:DatatypeProperty rdf:about="https://w3id.org/ontoim/value">
        <rdfs:subPropertyOf rdf:resource="https://w3id.org/italia/onto/MU/value"/>
        <rdfs:domain rdf:resource="http://www.w3.org/2002/07/owl#Thing"/>
        <rdfs:range rdf:resource="http://www.w3.org/2001/XMLSchema#nonNegativeInteger"/>
        <rdfs:label xml:lang="it">valore</rdfs:label>
        <rdfs:label xml:lang="en">value</rdfs:label>
    </owl:DatatypeProperty>
    


    <!-- 
    ///////////////////////////////////////////////////////////////////////////////////////
    //
    // Classes
    //
    ///////////////////////////////////////////////////////////////////////////////////////
     -->

    


    <!-- https://w3id.org/ontoim/AccessiblePointOfInterest -->

    <owl:Class rdf:about="https://w3id.org/ontoim/AccessiblePointOfInterest">
        <rdfs:subClassOf rdf:resource="https://w3id.org/italia/onto/POI/PointOfInterest"/>
        <rdfs:subClassOf>
            <owl:Restriction>
                <owl:onProperty rdf:resource="https://w3id.org/italia/onto/ACCO/hasOfferedServiceDescription"/>
                <owl:allValuesFrom rdf:resource="https://w3id.org/italia/onto/ACCO/OfferedServiceDescription"/>
            </owl:Restriction>
        </rdfs:subClassOf>
        <rdfs:subClassOf>
            <owl:Restriction>
                <owl:onProperty rdf:resource="https://w3id.org/italia/onto/AccessCondition/hasAccessCondition"/>
                <owl:allValuesFrom rdf:resource="https://w3id.org/italia/onto/AccessCondition/AccessCondition"/>
            </owl:Restriction>
        </rdfs:subClassOf>
        <rdfs:subClassOf>
            <owl:Restriction>
                <owl:onProperty rdf:resource="https://w3id.org/ontoim/ownedBy"/>
                <owl:allValuesFrom rdf:resource="https://w3id.org/italia/onto/COV/Organization"/>
            </owl:Restriction>
        </rdfs:subClassOf>
        <rdfs:subClassOf>
            <owl:Restriction>
                <owl:onProperty rdf:resource="https://w3id.org/italia/onto/SM/hasOnlineContactPoint"/>
                <owl:maxQualifiedCardinality rdf:datatype="http://www.w3.org/2001/XMLSchema#nonNegativeInteger">1</owl:maxQualifiedCardinality>
                <owl:onClass rdf:resource="https://w3id.org/italia/onto/SM/OnlineContactPoint"/>
            </owl:Restriction>
        </rdfs:subClassOf>
        <rdfs:subClassOf>
            <owl:Restriction>
                <owl:onProperty rdf:resource="https://w3id.org/italia/onto/SM/hasPhysicalContactPoint"/>
                <owl:maxQualifiedCardinality rdf:datatype="http://www.w3.org/2001/XMLSchema#nonNegativeInteger">1</owl:maxQualifiedCardinality>
                <owl:onClass rdf:resource="https://w3id.org/italia/onto/SM/PhysicalContactPoint"/>
            </owl:Restriction>
        </rdfs:subClassOf>
        <rdfs:comment xml:lang="en">An Accessible Point of Interest is a Point of Interest, usually a building, a shopping center, a pharmacy, etc.... It inherits the properties of OntoPiA&apos;s Point of Interest, but it also has an online or physical contact point, access conditions, offered services descriptions and an owner (Organization).</rdfs:comment>
        <rdfs:comment xml:lang="it">Un Punto di Interesse Accessibile è un Punto di Interesse, solitamente un edificio, un centro commerciale, una farmacia ecc.... Eredita le proprietà del Punto di Interesse di OntoPiA, ma possiede anche un punto di contatto online o fisico, una o più condizioni di acceso, può avere dei servizi generici e ha un possessore (Organizzazione).</rdfs:comment>
        <rdfs:label xml:lang="en">Accessible Point of Interest</rdfs:label>
        <rdfs:label xml:lang="it">Punto di Interesse Accessibile</rdfs:label>
    </owl:Class>
    


    <!-- https://w3id.org/ontoim/AssociationCategory -->

    <owl:Class rdf:about="https://w3id.org/ontoim/AssociationCategory">
        <rdfs:subClassOf rdf:resource="https://w3id.org/italia/onto/l0/Topic"/>
    </owl:Class>
    


    <!-- https://w3id.org/ontoim/Booking -->

    <owl:Class rdf:about="https://w3id.org/ontoim/Booking">
        <rdfs:subClassOf rdf:resource="https://w3id.org/ontoim/DemographicEvent"/>
        <rdfs:comment xml:lang="it">Questa classe rappresenta un evento demografico di prenotazioni in una struttura ricettiva.</rdfs:comment>
        <rdfs:comment xml:lang="en">This class represents a demographic event of bookins to an accommodation facility.</rdfs:comment>
        <rdfs:label xml:lang="en">Booking</rdfs:label>
        <rdfs:label xml:lang="it">Prenotazione</rdfs:label>
    </owl:Class>
    


    <!-- https://w3id.org/ontoim/Bookings -->

    <owl:Class rdf:about="https://w3id.org/ontoim/Bookings">
        <rdfs:subClassOf rdf:resource="https://w3id.org/ontoim/DemographicObservation"/>
        <rdfs:comment xml:lang="it">Questa classe rappresenta un&apos;osservazione demografica sui turisti prenotati in una struttura ricettiva.</rdfs:comment>
        <rdfs:comment xml:lang="en">This class represents a demographic observation on the tourists booked in an accommodation facility.</rdfs:comment>
        <rdfs:label xml:lang="en">Bookings</rdfs:label>
        <rdfs:label xml:lang="it">Prenotazioni</rdfs:label>
    </owl:Class>
    


    <!-- https://w3id.org/ontoim/Citizens -->

    <owl:Class rdf:about="https://w3id.org/ontoim/Citizens">
        <rdfs:subClassOf rdf:resource="https://w3id.org/ontoim/DemographicObservation"/>
        <rdfs:comment xml:lang="it">Questa classe rappresenta un&apos;osservazione demografica fatta sui cittadini. Ad esempio, il numero di cittadini presenti nel comune.</rdfs:comment>
        <rdfs:comment xml:lang="en">This class represents a demographic observation made on the citizens. E.g. the number of citizens in the municipality.</rdfs:comment>
        <rdfs:label xml:lang="en">Citizens</rdfs:label>
        <rdfs:label xml:lang="it">Cittadini</rdfs:label>
    </owl:Class>
    


    <!-- https://w3id.org/ontoim/CivilStatus -->

    <owl:Class rdf:about="https://w3id.org/ontoim/CivilStatus">
        <rdfs:subClassOf rdf:resource="https://w3id.org/ontoim/DemographicObservation"/>
        <rdfs:subClassOf>
            <owl:Restriction>
                <owl:onProperty rdf:resource="https://w3id.org/ontoim/hasCivilStatusCategory"/>
                <owl:qualifiedCardinality rdf:datatype="http://www.w3.org/2001/XMLSchema#nonNegativeInteger">1</owl:qualifiedCardinality>
                <owl:onClass rdf:resource="https://w3id.org/ontoim/CivilStatusCategory"/>
            </owl:Restriction>
        </rdfs:subClassOf>
        <rdfs:comment xml:lang="it">Questa classe rappresenta il numero di eventi di stato civile (nascite, matrimoni, morti, ecc...)</rdfs:comment>
        <rdfs:comment xml:lang="en">This class represents the number of civil status events and their types (marriages, births, deaths, etc...)</rdfs:comment>
        <rdfs:label xml:lang="en">Civil Status</rdfs:label>
        <rdfs:label xml:lang="it">Stato Civile</rdfs:label>
    </owl:Class>
    


    <!-- https://w3id.org/ontoim/CivilStatusCategory -->

    <owl:Class rdf:about="https://w3id.org/ontoim/CivilStatusCategory">
        <rdfs:subClassOf rdf:resource="https://w3id.org/italia/onto/l0/Topic"/>
        <rdfs:comment xml:lang="it">Questa classe rappresenta la categoria dell&apos;evento di stato civile. Gli elementi di questa classe sono di tipo skos:Concept e devono essere definiti secondo il vocabolario controllato disponibile a https://w3id.org/ontoim/controlled-vocabulary/civil-status-categories</rdfs:comment>
        <rdfs:comment xml:lang="en">This class represents the category of the civil status event. The elements of this class are skos:Concept and must be defined according to the controlled vocabulary available at https://w3id.org/ontoim/controlled-vocabulary/civil-status-categories</rdfs:comment>
        <rdfs:label xml:lang="it">Categoria di Stato Civile</rdfs:label>
        <rdfs:label xml:lang="en">Civil Status Category</rdfs:label>
    </owl:Class>
    


    <!-- https://w3id.org/ontoim/CivilStatusEvent -->

    <owl:Class rdf:about="https://w3id.org/ontoim/CivilStatusEvent">
        <rdfs:subClassOf rdf:resource="https://w3id.org/ontoim/DemographicEvent"/>
        <rdfs:subClassOf>
            <owl:Restriction>
                <owl:onProperty rdf:resource="https://w3id.org/ontoim/hasCivilStatusCategory"/>
                <owl:qualifiedCardinality rdf:datatype="http://www.w3.org/2001/XMLSchema#nonNegativeInteger">1</owl:qualifiedCardinality>
                <owl:onClass rdf:resource="https://w3id.org/ontoim/CivilStatusCategory"/>
            </owl:Restriction>
        </rdfs:subClassOf>
        <rdfs:comment xml:lang="it">Questa classe rappresenta un evento di stato civile, come una nascita, un decesso, un matrimonio ecc...</rdfs:comment>
        <rdfs:comment xml:lang="en">This class represents a civil status event, like a birth, a death, a marriage etc...</rdfs:comment>
        <rdfs:label xml:lang="en">Civil Status Event</rdfs:label>
        <rdfs:label xml:lang="it">Evento di Stato Civile</rdfs:label>
    </owl:Class>
    


    <!-- https://w3id.org/ontoim/CompanyDemographicCategory -->

    <owl:Class rdf:about="https://w3id.org/ontoim/CompanyDemographicCategory">
        <rdfs:subClassOf rdf:resource="https://w3id.org/italia/onto/l0/Topic"/>
    </owl:Class>
    


    <!-- https://w3id.org/ontoim/DemographicEvent -->

    <owl:Class rdf:about="https://w3id.org/ontoim/DemographicEvent">
        <rdfs:subClassOf rdf:resource="https://w3id.org/italia/onto/l0/EventOrSituation"/>
        <rdfs:subClassOf>
            <owl:Restriction>
                <owl:onProperty rdf:resource="https://w3id.org/ontoim/hasDemographicReference"/>
                <owl:maxQualifiedCardinality rdf:datatype="http://www.w3.org/2001/XMLSchema#nonNegativeInteger">1</owl:maxQualifiedCardinality>
                <owl:onClass rdf:resource="https://w3id.org/italia/onto/CPV/Person"/>
            </owl:Restriction>
        </rdfs:subClassOf>
        <rdfs:subClassOf>
            <owl:Restriction>
                <owl:onProperty rdf:resource="https://w3id.org/ontoim/hasSpatialDelimitation"/>
                <owl:maxQualifiedCardinality rdf:datatype="http://www.w3.org/2001/XMLSchema#nonNegativeInteger">1</owl:maxQualifiedCardinality>
                <owl:onClass rdf:resource="https://w3id.org/italia/onto/CLV/SpatialObject"/>
            </owl:Restriction>
        </rdfs:subClassOf>
        <rdfs:subClassOf>
            <owl:Restriction>
                <owl:onProperty rdf:resource="https://w3id.org/italia/onto/TI/date"/>
                <owl:qualifiedCardinality rdf:datatype="http://www.w3.org/2001/XMLSchema#nonNegativeInteger">1</owl:qualifiedCardinality>
                <owl:onDataRange rdf:resource="http://www.w3.org/2001/XMLSchema#dateTime"/>
            </owl:Restriction>
        </rdfs:subClassOf>
        <rdfs:comment xml:lang="it">Questa classe rappresenta una versione non aggregata delle osservazioni demografiche, dove gli eventi di stato civile, le prenotazioni, le iscrizioni sono separate. Ogni evento demografico rappresenta un evento (es: nascita, matrimonio) in un certo istante e in una delimitazione spaziale.</rdfs:comment>
        <rdfs:comment xml:lang="en">This class represents a non-aggregated version of the demographic observations, where the civil status events, the bookings or subscriptions are separated. Each demographic event represents a single event (e.g. a birth, a marriage) at a certain time and in a spatial delimitation.</rdfs:comment>
        <rdfs:label xml:lang="en">Demographic Event</rdfs:label>
        <rdfs:label xml:lang="it">Evento Demografico</rdfs:label>
    </owl:Class>
    


    <!-- https://w3id.org/ontoim/DemographicObservation -->

    <owl:Class rdf:about="https://w3id.org/ontoim/DemographicObservation">
        <rdfs:subClassOf rdf:resource="https://w3id.org/italia/onto/l0/Activity"/>
        <rdfs:subClassOf>
            <owl:Restriction>
                <owl:onProperty rdf:resource="https://w3id.org/italia/onto/TI/hasTemporalEntity"/>
                <owl:maxQualifiedCardinality rdf:datatype="http://www.w3.org/2001/XMLSchema#nonNegativeInteger">1</owl:maxQualifiedCardinality>
                <owl:onClass rdf:resource="https://w3id.org/italia/onto/TI/TemporalEntity"/>
            </owl:Restriction>
        </rdfs:subClassOf>
        <rdfs:subClassOf>
            <owl:Restriction>
                <owl:onProperty rdf:resource="https://w3id.org/ontoim/hasDemographicReference"/>
                <owl:maxQualifiedCardinality rdf:datatype="http://www.w3.org/2001/XMLSchema#nonNegativeInteger">1</owl:maxQualifiedCardinality>
                <owl:onClass>
                    <owl:Class>
                        <owl:unionOf rdf:parseType="Collection">
                            <rdf:Description rdf:about="https://w3id.org/italia/onto/CPV/Family"/>
                            <rdf:Description rdf:about="https://w3id.org/italia/onto/CPV/Person"/>
                        </owl:unionOf>
                    </owl:Class>
                </owl:onClass>
            </owl:Restriction>
        </rdfs:subClassOf>
        <rdfs:subClassOf>
            <owl:Restriction>
                <owl:onProperty rdf:resource="https://w3id.org/ontoim/hasSpatialDelimitation"/>
                <owl:maxQualifiedCardinality rdf:datatype="http://www.w3.org/2001/XMLSchema#nonNegativeInteger">1</owl:maxQualifiedCardinality>
                <owl:onClass rdf:resource="https://w3id.org/italia/onto/CLV/SpatialObject"/>
            </owl:Restriction>
        </rdfs:subClassOf>
        <rdfs:subClassOf>
            <owl:Restriction>
                <owl:onProperty rdf:resource="https://w3id.org/ontoim/value"/>
                <owl:qualifiedCardinality rdf:datatype="http://www.w3.org/2001/XMLSchema#nonNegativeInteger">1</owl:qualifiedCardinality>
                <owl:onDataRange rdf:resource="http://www.w3.org/2001/XMLSchema#nonNegativeInteger"/>
            </owl:Restriction>
        </rdfs:subClassOf>
        <rdfs:comment xml:lang="en">A demographic observation is an observation made on the population of an entity, which can be the municipality, an organization, an event... The value defines the quantity of people or families observed, while the demographic reference represents the characteristics of the people observed. The demographic observation has also time and space delimitation. An example can be the number of female population of the municipality in 2021, or the number of italian citizens for a specific geographical area in 2020.</rdfs:comment>
        <rdfs:comment xml:lang="it">Un&apos;osservazione demografica è un&apos;osservazione fatta sulla popolazione di un&apos;entità, che può essere il comune, un&apos;organizzazione o un evento. Il valore definisce la quantità di persone o famiglie osservate, mentre il riferimento demografico rappresenta le caratteristiche osservate. L&apos;osservazione demografica ha inoltre una un tempo e uno spazio limitato. Ad esempio, può essere il numero di donne nel comune nel 2021, o il numero di cittadini italiani in una specifica area geografica nel 2020.</rdfs:comment>
        <rdfs:label xml:lang="en">Demographic Observation</rdfs:label>
        <rdfs:label xml:lang="it">Osservazione Demografica</rdfs:label>
    </owl:Class>
    


    <!-- https://w3id.org/ontoim/Employees -->

    <owl:Class rdf:about="https://w3id.org/ontoim/Employees">
        <rdfs:subClassOf rdf:resource="https://w3id.org/ontoim/DemographicObservation"/>
        <rdfs:comment xml:lang="it">Questa classe rappresenta un&apos;osservazione demografica sui dipendenti di un&apos;impresa.</rdfs:comment>
        <rdfs:comment xml:lang="en">This class represents a demographic observation on the employees of an organization.</rdfs:comment>
        <rdfs:label xml:lang="it">Dipendenti</rdfs:label>
        <rdfs:label xml:lang="en">Employees</rdfs:label>
    </owl:Class>
    


    <!-- https://w3id.org/ontoim/Members -->

    <owl:Class rdf:about="https://w3id.org/ontoim/Members">
        <rdfs:subClassOf rdf:resource="https://w3id.org/ontoim/DemographicObservation"/>
        <rdfs:comment xml:lang="it">Questa classe rappresenta un&apos;osservazione demografica sui membri di un&apos;associazione.</rdfs:comment>
        <rdfs:comment xml:lang="en">This class represents a demographic observation on the members of an association.</rdfs:comment>
        <rdfs:label xml:lang="en">Members</rdfs:label>
        <rdfs:label xml:lang="it">Membri</rdfs:label>
    </owl:Class>
    


    <!-- https://w3id.org/ontoim/Organization -->

    <owl:Class rdf:about="https://w3id.org/ontoim/Organization">
        <rdfs:subClassOf rdf:resource="https://w3id.org/italia/onto/COV/Organization"/>
        <rdfs:subClassOf>
            <owl:Restriction>
                <owl:onProperty rdf:resource="https://w3id.org/ontoim/hasEmployees"/>
                <owl:allValuesFrom rdf:resource="https://w3id.org/ontoim/Employees"/>
            </owl:Restriction>
        </rdfs:subClassOf>
        <rdfs:subClassOf>
            <owl:Restriction>
                <owl:onProperty rdf:resource="https://w3id.org/ontoim/hasLocalUnitAddress"/>
                <owl:allValuesFrom rdf:resource="https://w3id.org/italia/onto/CLV/Address"/>
            </owl:Restriction>
        </rdfs:subClassOf>
        <rdfs:subClassOf>
            <owl:Restriction>
                <owl:onProperty rdf:resource="https://w3id.org/ontoim/providesService"/>
                <owl:allValuesFrom rdf:resource="https://w3id.org/italia/onto/CPSV/Service"/>
            </owl:Restriction>
        </rdfs:subClassOf>
        <rdfs:subClassOf>
            <owl:Restriction>
                <owl:onProperty rdf:resource="https://w3id.org/ontoim/endActivityDate"/>
                <owl:maxQualifiedCardinality rdf:datatype="http://www.w3.org/2001/XMLSchema#nonNegativeInteger">1</owl:maxQualifiedCardinality>
                <owl:onDataRange rdf:resource="http://www.w3.org/2001/XMLSchema#date"/>
            </owl:Restriction>
        </rdfs:subClassOf>
        <rdfs:subClassOf>
            <owl:Restriction>
                <owl:onProperty rdf:resource="https://w3id.org/ontoim/liquidationDate"/>
                <owl:maxQualifiedCardinality rdf:datatype="http://www.w3.org/2001/XMLSchema#nonNegativeInteger">1</owl:maxQualifiedCardinality>
                <owl:onDataRange rdf:resource="http://www.w3.org/2001/XMLSchema#date"/>
            </owl:Restriction>
        </rdfs:subClassOf>
    </owl:Class>
    


    <!-- https://w3id.org/ontoim/OrganizationSection -->

    <owl:Class rdf:about="https://w3id.org/ontoim/OrganizationSection">
        <rdfs:subClassOf rdf:resource="https://w3id.org/italia/onto/l0/Topic"/>
    </owl:Class>
    


    <!-- https://w3id.org/ontoim/PrivateOrganization -->

    <owl:Class rdf:about="https://w3id.org/ontoim/PrivateOrganization">
        <rdfs:subClassOf rdf:resource="https://w3id.org/italia/onto/COV/PrivateOrganization"/>
        <rdfs:subClassOf rdf:resource="https://w3id.org/ontoim/Organization"/>
    </owl:Class>
    


    <!-- https://w3id.org/ontoim/Subscriber -->

    <owl:Class rdf:about="https://w3id.org/ontoim/Subscriber">
        <rdfs:subClassOf rdf:resource="https://w3id.org/ontoim/DemographicEvent"/>
        <rdfs:comment xml:lang="it">Questa classe rappresenta un evento demografico di iscritti a un evento, una scuola o un corso.</rdfs:comment>
        <rdfs:comment xml:lang="en">This class represents a demographic event of subscribers to an event, a school or a course.</rdfs:comment>
        <rdfs:label xml:lang="it">Iscritto</rdfs:label>
        <rdfs:label xml:lang="en">Subscriber</rdfs:label>
    </owl:Class>
    


    <!-- https://w3id.org/ontoim/Subscribers -->

    <owl:Class rdf:about="https://w3id.org/ontoim/Subscribers">
        <rdfs:subClassOf rdf:resource="https://w3id.org/ontoim/DemographicObservation"/>
        <rdfs:comment xml:lang="it">Questa classe rappresenta un&apos;osservazione demografica sugli iscritti ad un evento, una scuola o un corso.</rdfs:comment>
        <rdfs:comment xml:lang="en">This class represents a demographic observation on the subscrivers to an event, a school or a course.</rdfs:comment>
        <rdfs:label xml:lang="it">Iscritti</rdfs:label>
        <rdfs:label xml:lang="en">Subscribers</rdfs:label>
    </owl:Class>
    


    <!-- https://w3id.org/ontoim/TouristType -->

    <owl:Class rdf:about="https://w3id.org/ontoim/TouristType">
        <owl:equivalentClass>
            <owl:Class>
                <owl:oneOf rdf:parseType="Collection">
                    <rdf:Description rdf:about="https://w3id.org/ontoim/Arrival"/>
                    <rdf:Description rdf:about="https://w3id.org/ontoim/Presence"/>
                </owl:oneOf>
            </owl:Class>
        </owl:equivalentClass>
        <rdfs:comment xml:lang="it">Questa classe è una classe numerata che rappresenta la tipologia di turista: arrivo o presenza.</rdfs:comment>
        <rdfs:comment xml:lang="en">This class is an enumerated class representing the typology of tourist: arrival or presence.</rdfs:comment>
        <rdfs:label xml:lang="it">Tipo di Turista</rdfs:label>
        <rdfs:label xml:lang="en">Tourist Type</rdfs:label>
    </owl:Class>
    


    <!-- https://w3id.org/ontoim/Tourists -->

    <owl:Class rdf:about="https://w3id.org/ontoim/Tourists">
        <rdfs:subClassOf rdf:resource="https://w3id.org/ontoim/DemographicObservation"/>
        <rdfs:subClassOf>
            <owl:Restriction>
                <owl:onProperty rdf:resource="https://w3id.org/ontoim/hasTouristType"/>
                <owl:maxQualifiedCardinality rdf:datatype="http://www.w3.org/2001/XMLSchema#nonNegativeInteger">1</owl:maxQualifiedCardinality>
                <owl:onClass rdf:resource="https://w3id.org/ontoim/TouristType"/>
            </owl:Restriction>
        </rdfs:subClassOf>
        <rdfs:comment xml:lang="it">Questa classe rappresenta un&apos;osservazione demografica sui turisti. Le osservazioni sui turisti è divisa in arrivi e presenze.</rdfs:comment>
        <rdfs:comment xml:lang="en">This class represents the demographic observation for tourism. Tourism observation is divided in arrivals and presences.</rdfs:comment>
        <rdfs:label xml:lang="en">Tourists</rdfs:label>
        <rdfs:label xml:lang="it">Turisti</rdfs:label>
    </owl:Class>
    


    <!-- 
    ///////////////////////////////////////////////////////////////////////////////////////
    //
    // Individuals
    //
    ///////////////////////////////////////////////////////////////////////////////////////
     -->

    


    <!-- https://www.dei.unipd.it -->

    <owl:NamedIndividual rdf:about="https://www.dei.unipd.it">
        <rdfs:label rdf:datatype="http://www.w3.org/2000/01/rdf-schema#Literal">Università di Padova</rdfs:label>
        <sdo:name xml:lang="en">University of Padova, Department of Information Engineering</sdo:name>
        <sdo:name xml:lang="it">Università degli Studi di Padova, Dipartimento di Ingegneria dell&apos;Informazione</sdo:name>
        <sdo:url rdf:resource="https://www.dei.unipd.it"/>
    </owl:NamedIndividual>
    


    <!-- https://orcid.org/0000-0002-6249-0899 -->

    <owl:NamedIndividual rdf:about="https://orcid.org/0000-0002-6249-0899">
        <rdfs:label>Luca Martinelli</rdfs:label>
        <sdo:affiliation rdf:resource="https://www.dei.unipd.it"/>
        <sdo:email rdf:resource="mailto:luca.martinelli.1@studenti.unipd.it"/>
        <sdo:identifier rdf:resource="https://orcid.org/0000-0002-6249-0899"/>
        <sdo:name>Luca Martinelli</sdo:name>
    </owl:NamedIndividual>
    


    <!-- https://w3id.org/ontoim/Arrival -->

    <owl:NamedIndividual rdf:about="https://w3id.org/ontoim/Arrival">
        <rdf:type rdf:resource="https://w3id.org/ontoim/TouristType"/>
        <rdfs:label xml:lang="en">Arrival</rdfs:label>
        <rdfs:label xml:lang="it">Arrivo</rdfs:label>
    </owl:NamedIndividual>
    


    <!-- https://w3id.org/ontoim/Presence -->

    <owl:NamedIndividual rdf:about="https://w3id.org/ontoim/Presence">
        <rdf:type rdf:resource="https://w3id.org/ontoim/TouristType"/>
        <rdfs:label xml:lang="en">Presence</rdfs:label>
        <rdfs:label xml:lang="it">Presenza</rdfs:label>
    </owl:NamedIndividual>
</rdf:RDF>



<!-- Generated by the OWL API (version 4.5.9.2019-02-01T07:24:44Z) https://github.com/owlcs/owlapi -->

